fixed #68

theories/Debugger.v
@@ -5,26 +5,49 @@ Require Import Strings.String.
 
 Definition Break : Exception. exact exception. Qed.
 
-Definition debug {A:Type} (bks : list dyn) : M A -> M unit :=
+Definition isReduce {A} (x:A) : M bool :=
+  mmatch x with
+  | [? T r t1 t2] let x := reduce r t1 : T in t2 x => M.ret true
+  | _ => M.ret false
+  end.
+
+Definition debug (trace: bool) {A:Type} (bks : list dyn) : M A -> M unit :=
   M.break (fun A (x:A) =>
-             let x := reduce (RedWhd [rl:RedBeta;RedMatch;RedFix;RedZeta]) x in
              v <- M.decompose x;
              let (hd, _) := v in
-             mif M.find (fun d=>M.unify_cumul d hd UniMatchNoRed) bks then
+             let (_, hd) := hd : dyn in
+             mif isReduce hd then (* avoid computation of reduce *)
                M.print_term x;;
-               inp <- M.read_line;
-               match inp with
-               | "e" => M.raise Break
-               | _ => M.ret x
-               end
-             else M.ret x).
+               M.ret x
+             else
+               let x := reduce (RedWhd [rl:RedBeta;RedMatch;RedFix;RedZeta]) x in
+               v <- M.decompose x;
+               let (hd, _) := v in
+               mif M.find (fun d=>M.unify_cumul d hd UniMatchNoRed) bks then
+                 M.print_term x;;
+                 inp <- M.read_line;
+                 match inp with
+                 | "e" => M.raise Break
+                 | _ => M.ret x
+                 end
+               else if trace then
+                      M.print_term x;; M.ret x
+                    else M.ret x).
 
-Definition debugT {A} (bks : list dyn) (t: gtactic A) : gtactic unit := fun g=>
-  debug bks (t g) ;; M.ret nil.
+Definition debugT {A} (trace: bool) (bks : list dyn) (t: gtactic A) : gtactic unit := fun g=>
+  debug trace bks (t g) ;; M.ret nil.
 Import Mtac2.List.ListNotations.
 
 
 Definition test : True.
 MProof.
-  debugT [m: (*HAVE FUN Dyn (@M.ret) | Dyn (@M.unify) *)] (T.apply I).
+  debugT false [m: (*HAVE FUN Dyn (@M.ret) | Dyn (@M.unify) *)] (T.apply I).
 Qed.
+
+Goal unit.
+MProof.
+  (* Prints `6` *)
+  Fail (let x := reduce (RedStrong RedAll) (3+3) in M.print_term x;; M.failwith "").
+  (* Prints `rbcv (3+3)` *)
+  Fail (debug true [m:Dyn (@M.ret)] (let x := reduce (RedStrong RedAll) (3+3) in M.print_term x;; M.failwith "")).
+Abort.
